block out all the shifting lemmas

LeanScratch/Untyped/ConfluenceBeta.lean
@@ -1,7 +1,38 @@
 import LeanScratch.Untyped.Basic
-import LeanScratch.Untyped.Parallel
 import LeanScratch.Untyped.Reduction
+import LeanScratch.Untyped.Shifting
 import LeanScratch.Untyped.Beta
+
+open Term
+
+inductive Parallel : Term → Term → Prop
+| var (x : ℕ) : Parallel (var x) (var x)
+| abs {N N'} : Parallel N N' →  Parallel (abs N) (abs N')
+| app {L L' M M'} : Parallel L L' → Parallel M M' → Parallel {{{ ~L ~M }}} {{{ ~L' ~M' }}}
+| beta {N N' M M'} : Parallel N N' → Parallel M M' → Parallel {{{ (λ . ~M) ~N }}} (M' [0 := N'.shift]).unshift
+
+notation:39 t " ⇉ "  t' =>                       Parallel t t'
+notation:39 t " ⇉* " t' => Relation.ReflTransGen Parallel t t'
+
+@[refl]
+theorem Parallel.refl (M : Term) : (M ⇉ M) := by
+  induction M
+  case var x => exact Parallel.var x
+  case abs body ih => exact Parallel.abs ih
+  case app l r l_ih r_ih => exact Parallel.app l_ih r_ih
+
+theorem para_shift {c d : ℕ} {M M'} : (M ⇉ M') → (M.shiftₙ c d ⇉ M'.shiftₙ c d) := by
+  intros para
+  revert c d
+  induction para <;> intros c d
+  case var x => rfl
+  case app => constructor <;> aesop
+  case abs => constructor; aesop
+  case beta t2 t2' t1 t1' t1p t2p ih₁ ih₂ =>
+    simp [shiftₙ]
+    rw [shiftUnshiftSwap ?_ (betaShifted' 0 t1' t2'), shiftSubstSwap, ←shiftShiftSwap]
+    exact Parallel.beta ih₁ ih₂
+    all_goals linarith
 
 lemma step_to_para {M N} (step : M →β N) : (M ⇉ N) := by
   induction step 
@@ -34,5 +65,112 @@ theorem parachain_iff_redex {M N} : (M ⇉* N) ↔ (M ↠β N) := by
   refine Iff.intro ?chain_to_redex ?redex_to_chain <;> intros h <;> induction' h <;> try rfl
   case redex_to_chain.tail redex chain => exact Relation.ReflTransGen.tail chain (step_to_para redex)
   case chain_to_redex.tail para  redex => exact Relation.ReflTransGen.trans redex (para_to_redex para)
+
+open Shifted Step_R in
+theorem beta_shift_conserve  : ∀ {d c t1 t2}, (t1 →β t2) → Shifted d c t1 → Shifted d c t2 := by
+  intros d c t1 t2 step s
+  match step, s with
+  | ξ  p, sabs s1 => exact sabs (beta_shift_conserve p s1)
+  | ξₗ p, sapp s1 s2 => exact sapp s1 (beta_shift_conserve p s2)
+  | ξᵣ p, sapp s1 s2 => exact sapp (beta_shift_conserve p s1) s2
+  | reduce (β.reduce), (sapp (sabs s1) s2) => 
+      have bs := @betaShifted2 d c 0
+      simp at bs
+      rw [Nat.add_comm] at bs
+      exact bs s1 s2
+
+theorem redex_shift_conserve : ∀ {d c t1 t2}, (t1 ↠β t2) → Shifted d c t1 → Shifted d c t2 := by
+  intros d c t1 t2 redex s
+  induction' redex
+  case refl => assumption
+  case tail a a_ih => exact beta_shift_conserve a a_ih
+
+theorem para_shift_conserve  : ∀ {d c t1 t2}, (t1 ⇉  t2) → Shifted d c t1 → Shifted d c t2 := by
+  intros d c t1 t2 para s
+  exact redex_shift_conserve (para_to_redex para) s
+
+theorem para_unshift {c d} {M M'} : (M ⇉ M') → Shifted d c M → (M.unshiftₙ c d ⇉ M'.unshiftₙ c d) := by
+  intros para sM
+  match para, sM with
+  | Parallel.var _, _ => rfl
+  | Parallel.app l r, Shifted.sapp sl sr => exact Parallel.app (para_unshift l sl) (para_unshift r sr)
+  | Parallel.abs body, Shifted.sabs sbody => exact Parallel.abs (para_unshift body sbody)
+  | Parallel.beta r2 r1, Shifted.sapp (Shifted.sabs s1) s2 => 
+      simp [shiftₙ]
+      rename_i X Y Z W
+      have s1' := para_shift_conserve r1 s1
+      have s2' := para_shift_conserve r2 s2
+
+      rw [unshiftUnshiftSwap (by linarith) (betaShifted' 0 W Y) ?com_shift]
+      case com_shift =>
+        have bshift := @betaShifted2 d c 0
+        rw [Nat.zero_add, Nat.zero_add, Nat.add_comm] at bshift
+        exact bshift s1' s2'
+
+      rw [unshiftSubstSwap2 (by linarith) s1' ?com_shift]
+      case com_shift =>
+        rw [Nat.add_comm]
+        refine shiftShifted' (by linarith) s2'        
+
+      rw [←unshiftShiftSwap (by linarith) s2']
+
+      exact Parallel.beta (para_unshift r2 s2) (para_unshift r1 s1)  
+
+theorem sub_para {x : ℕ} {N N' M M'} : (N ⇉ N') → (M ⇉ M') → (N [x := M] ⇉ N' [x := M']) := by
+  intros N_N' M_M'
+  match N_N' with
+  | Parallel.abs r1 => exact Parallel.abs (sub_para r1 (para_shift M_M'))
+  | Parallel.var x =>
+      simp [sub]
+      rename_i x'
+      by_cases eq : x = x' <;> simp [eq]
+      · exact M_M'
+      · rfl
+  | Parallel.app l r =>
+      apply Parallel.app
+      apply sub_para l
+      exact M_M'
+      apply sub_para
+      exact r
+      exact M_M'
+  | Parallel.beta r2 r1 => 
+      rename_i X W Y Z
+      simp [shift, unshift]
+      have eq : ((unshiftₙ 0 1 (Z[0:=shiftₙ 0 1 W]))[x:=M']) 
+                = 
+                (unshiftₙ 0 1 ((Z [x+1 := shiftₙ 0 1 M']) [0 := shiftₙ 0 1 (W [x := M'])]))
+                := by
+          rw [←unshiftSubstSwap' _ _ (betaShifted' 0 Z W)]
+          have sss := substSubstSwap x 0 Z W M'
+          rw [Nat.zero_add, Nat.add_comm 1 x] at sss
+          rw [sss]
+      rw [eq]
+      refine Parallel.beta (sub_para r2 M_M') (sub_para r1 (para_shift M_M'))
+
+def Term.plus (t : Term) : Term :=
+  match t with
+  | var x => var x
+  | abs N => abs N.plus
+  | app (abs N) M => (N.plus [0 := M.plus.shift]).unshift
+  | app L M => app L.plus M.plus
+
+theorem para_tri {M N} (para : M ⇉ N) : (N ⇉ M.plus) := 
+  match para with
+  | Parallel.var x => Parallel.var x
+  | Parallel.abs ρ => Parallel.abs (para_tri ρ)
+  | Parallel.beta p1 p2 => by
+      refine para_unshift (sub_para (para_tri p2) (para_shift (para_tri p1))) ?_
+      simp [sub]
+      apply betaShifted'
+  | @Parallel.app (Term.abs _) _ _ _ (Parallel.abs p1) p2 => Parallel.beta (para_tri p2) (para_tri p1)
+  | @Parallel.app (var _) _ _ _ p1 p2 => Parallel.app (para_tri p1) (para_tri p2)
+  | @Parallel.app (app _ _) _ _ _ p1 p2 => Parallel.app (para_tri p1) (para_tri p2)
+
+theorem para_diamond : Diamond Parallel := by
+  simp [Diamond]
+  intros M N N' p1 p2
+  exact ⟨M.plus, ⟨para_tri p1, para_tri p2⟩⟩
+
+theorem para_confluence : Confluence Parallel := Relation.ReflTransGen.diamond para_diamond
 
 theorem confluence_beta : Confluence (· →β ·) := diamond_bisim parachain_iff_redex @para_confluence
